lecture11/exists-witness.dfy
@@ -5,4 +5,7 @@ predicate fitsBetween(x : int, lo : int, hi : int)
 }
 
 lemma exist1(j:int)
-  ensures exists i : int :: fitsBetween(i,2,4)
+  ensures exists i : int :: fitsBetween(i,2,4){
+    assert fitsBetween(3,2,4);
+    //assert exists i : int :: fitsBetween(i,2,4);
+  }
