lecture11/list-nth.dfy
@@ -13,4 +13,22 @@ function nth<T>(l : list<T>, n : nat) : T
 }
 
 lemma mem_nth(i : int, l : list<int>)
-  ensures member(i, l) <==> exists n : nat | n < length(l) :: nth(l,n) == i
+  ensures member(i, l) <==> exists idx : nat | idx < length(l) :: nth(l,idx) == i
+  {
+    match l case Nil =>{}
+    case Cons(j,js) =>{
+      if member(i,l){
+        if i == j {
+          assert nth(l,0) == i;
+        } else {
+          assert member(i,js);
+          var idx : nat :| idx < length(js) && nth(js,idx)==i;
+          assert nth(l,idx+1) == i;
+          assert idx+1 < length(l);
+          assert exists IDX : nat | IDX < length(l) :: nth(l,IDX) == i;
+        }
+      } else {
+
+      }
+    }
+  }
