lecture11/univ-recap.dfy
@@ -1,10 +1,20 @@
 predicate q(x:int)
-predicate r(x:int)
+predicate r(x:int){ true}
 
 lemma somename_arbitrary()
-  ensures forall x | 0 < x :: q(x)
+  ensures forall x | 0 < x :: q(x){
+    forall x ensures 0 < x ==> q(x){
+      if 0 < x{}
+    }
+  }
 
 
 lemma somename_instantiate(y:nat)
   requires forall x | 0 < x :: q(x)
   ensures r(y / 103)
+  {
+    if ( 0 < y) {
+      assert q(y);
+      assert r(y/103) by {}
+    }
+  }
